$\sum\limits_{i=0}^n(-1)^i\times C^i_n=?$

$1.\: n$ 为奇数

$\because C^m_n=C^{n-m}_n$

$\therefore \sum\limits_{i=0}^n(-1)^i\times C^i_n=0$

$2.\:m$ 为偶数

$\because C^m_n=C^{m-1}_{n-1}+C^{m}_{n-1}$

$\therefore \sum\limits_{i=0}^n(-1)^i\times C^i_n\\=C^0_n-(C^0_{n-1}+C^1_{n-1})+···-(C^{n-2}_{n-1}+C^{n-1}_{n-1})+C^{n}_n$

$\because C^0_n=C^n_n=C^0_{n-1}=C^{n-1}_{n-1}=1$

$\therefore $ 原式 $=0$



偶数项之和：

$\because \sum\limits^n_{m=0}C^m_n=2^n$

由上面得，奇数项之和 $=$ 偶数项之和 

$\therefore $ 偶数项之和 $=\frac{2^n}{2}\\=2^{n-1}$

