### è§£ç­” 4.3.1.2

$$
a_n=\sum\limits^n_{i=1}3^i(2i+1)^3,n\le10^9
\\=\sum\limits^n_{i=1}(2i+1)^33^i
\\ S_k=\sum\limits^n_{i=1}(2i+1)^k3^i
\\ 3S_3=\sum\limits^{n+1}_{i=1}(2i)^33^i
\\ 2S_3=\sum\limits^n_{i=1}((2i)^3-(2i+1)^3)3^i+(2(n+1))^33^{n+1}
\\ S_3=\frac{1}{2}\sum\limits^n_{i=1}(-12i^2-6i-1)3^i+(2n+2)^33^{n+1}
\\ S_2=\sum\limits^n_{i=1}(2i+1)^23^i
\\ 3S_2=\sum\limits^{n+1}_{i=1}(2i)^23^i
\\ 2S_2=\sum\limits^n_{i=1}((2i)^2-(2i+1)^2)3^i+(2(n+1))^23^{n+1}
\\ S_2=\frac{1}{2}\sum\limits^n_{i=1}(-4i-1)3^i+(2n+2)^23^{n+1}
\\ S_1=\sum\limits^n_{i=1}(2i+1)^13^i
\\ 3S_1=\sum\limits^{n+1}_{i=1}(2i)^13^i
\\ 2S_1=\sum\limits^n_{i=1}((2i)^1-(2i+1)^1)3^i+(2(n+1))^13^{n+1}
\\ S_1=\frac{1}{2}\sum\limits^n_{i=1}(-1)3^i+(2n+2)3^{n+1}
$$

