化简： $\sum\limits^{n}_{i=0}iC^{i}_{n}C^{i}_{m}$

由 $C^m_n=\sum\limits^{m}_{i=0}C^{i}_{p}C^{m-i}_{n-p}$ 可得：

$\sum\limits^{n}_{i=0}C^{i}_{n}C^{i}_{m}=C^{m}_{n+m}$

$\because C^m_n=C^{n-m}_n$

$\therefore \sum\limits^{n}_{i=0}iC^{i}_{n}C^{i}_{m}=\sum\limits^{n}_{i=0}iC^{n-i}_{n}C^{n-i}_{m}$

$\therefore 2\times \sum\limits^{n}_{i=0}iC^{i}_{n}C^{i}_{m}=\sum\limits^{n}_{i=0}nC^{i}_{n}C^{i}_{m}$

$\because \sum\limits^{n}_{i=0}nC^{i}_{n}C^{i}_{m}=n\times C^n_{n+m}$

$\therefore \sum\limits^{n}_{i=0}iC^{i}_{n}C^{i}_{m}=\frac{n\times C^n_{n+m}}{2}$

