### è§£ç­” 4.2.5.2

$\sum\limits^n_{i=1}i^32^i$

ä»¤ $S_k=\sum\limits^n_{i=1}i^k2^i$

åˆ™ $2S_3=\sum\limits^{n+1}_{i=1}(i-1)^32^i$

$2S_3-S_3=\sum\limits^{n}_{i=1}((i-1)^3-i^3)2^i+n^32^{n+1}$

$S_3=\sum\limits^n_{i=1}(-3i^2+3i-1)2^i+n^32^{n+1}$

$S_3=-3S_2+3S_1-(2^{n+1}-2)+n^32^{n+1}$

$2S_2=\sum\limits^{n+1}_{i=1}(i-1)^22^i$

$2S_2-S_2=\sum\limits^{n}_{i=1}((i-1)^2-i^2)2^i+n^22^{n+1}$

$S_2=\sum\limits^n_{i=1}(-2i+1)2^i+n^22^{n+1}$

$S_2=-2S_1+(2^{n+1}-2)+n^22^{n+1}$

$2S_1=\sum\limits^{n+1}_{i=1}(i-1)2^i$

$2S_1-S_1=\sum\limits^{n}_{i=1}((i-1)^1-i^1)2^i+n^12^{n+1}$
$$
S_1=\sum\limits^n_{i=1}(-2^i)+n2^{n+1}\\=-(2^{n+1}-2)+n2^{n+1}\\=2^{n+1}(n-1)+2
$$

$$
S_2=-2S_1+(2^{n+1}-2)+n^22^{n+1}
\\=-2\times(2^{n+1}(n-1)+2)+(2^{n+1}-2)+n^22^{n+1}
\\=2^{n+1}(n^2-2n+3)-6
$$

$$
S_3=-3S_2+3S_1-(2^{n+1}-2)+n^32^{n+1}
\\=-3(2^{n+1}(n^2-2n+3)-6)+3(2^{n+1}(n-1)+2)-(2^{n+1}-2)+n^32^{n+1}
\\=2^{n+1}\times(n^3-3n^2+9n-13)+26
$$

$$

$$
